proved some monotonicity properties of the abstract domain

rustfrontend/BorrowCheckDomain.v
@@ -2,6 +2,7 @@ Require Import Coqlib.
 Require Import Maps.
 Require Import AST.
 Require Import FSetWeakList DecidableType.
+Require Import FSetFacts.
 Require Import Lattice.
 Require Import Rusttypes Rustlight RustIR RustIRcfg.
 Require Import Ordered.
@@ -47,8 +48,9 @@ End Loan.
 (* May-live loan set *)
 Module LoanSet := FSetWeakList.Make(Loan).
 
-Module LoanSetL := LFSet(LoanSet).
+Module LoanSetFacts := FSetFacts.WFacts(LoanSet).
 
+Module LoanSetL := LFSet(LoanSet).
 
 (** Origin state *)
 
@@ -68,7 +70,6 @@ Definition eq (x y: t) :=
   | Dead, Dead => True
   | _, _ => False
   end.
-
   
 Lemma eq_refl: forall x, eq x x.
 Proof.
@@ -170,6 +171,25 @@ Qed.
 
 End LOrgSt.
 
+Global Instance LOrgSt_eq_equiv: 
+  Equivalence (LOrgSt.eq).
+Proof.
+  split.
+  red. eapply LOrgSt.eq_refl.
+  red. eapply LOrgSt.eq_sym.
+  red. eapply LOrgSt.eq_trans.
+Defined.
+
+
+Global Instance LOrgSt_lub_Proper:
+  Proper (LOrgSt.eq ==> LOrgSt.eq ==> LOrgSt.eq) LOrgSt.lub.
+Proof.
+  intros ls1 ls2 A ls3 ls4 B.
+  destruct ls1; destruct ls3; destruct ls2; destruct ls4; simpl in *.
+  all: try rewrite A; try rewrite B; try reflexivity.
+  all: try contradiction.
+Defined.  
+
 (** Lattice of disjoint-set mapping i.e., mapping of equivalent set
 represented by union-find structure *)
 
@@ -204,24 +224,34 @@ Proof.
     + rewrite PTree.gso; auto. apply L.eq_refl.
 Qed.
     
-Definition eq (x y: t) : Prop :=
-  forall p, L.eq (get p x) (get p y).
+Record eq' (x y: t) : Prop :=
+  { uf_eq: UFD.eq (uf x) (uf y);
+    m_eq: (forall p, L.eq (get p x) (get p y))}.
+
+Definition eq := eq'.
 
 Lemma eq_refl: forall x, eq x x.
 Proof.
-  unfold eq; intros. apply L.eq_refl.
+  intros. constructor.
+  eapply UFD.eq_refl.
+  intros. apply L.eq_refl.
 Qed.
 
 Lemma eq_sym: forall x y, eq x y -> eq y x.
 Proof.
-  unfold eq; intros. apply L.eq_sym; auto.
+  intros. inv H. constructor.  
+  eapply UFD.eq_sym. auto.
+  intros. apply L.eq_sym; auto.
 Qed.
 
 Lemma eq_trans: forall x y z, eq x y -> eq y z -> eq x z.
 Proof.
-  unfold eq; intros. eapply L.eq_trans; eauto.
+  intros. inv H; inv H0. constructor.
+  eapply UFD.eq_trans; eauto. 
+  intros. eapply L.eq_trans; eauto.
 Qed.
 
+(* unused *)
 Definition beq_elt (mx my: PTree.t L.t) (x y: positive) : bool :=
   match mx ! x, my ! y with
   | None, None => true
@@ -229,6 +259,7 @@ Definition beq_elt (mx my: PTree.t L.t) (x y: positive) : bool :=
   | _, _ => false
   end.
 
+(* unused *)
 Definition eqb_elt (dm1 dm2: t) a (v: UFD.vt) : bool :=
   (* the set of a in uf2 must be included in uf1 *)
   let x := (UFD.repr (uf dm1) a) in
@@ -237,6 +268,7 @@ Definition eqb_elt (dm1 dm2: t) a (v: UFD.vt) : bool :=
   (* the values of representative nodes are equal *)
   && beq_elt (m dm1) (m dm2) x y.
 
+(* unused *)
 Definition val_eqb_opt2 (m1: PTree.t L.t) (uf2: UFD.t) p (v2: L.t) : bool :=
   match (UFD.m uf2) ! p with
   (* p is a singleton in uf2 *)
@@ -250,7 +282,7 @@ Definition val_eqb_opt2 (m1: PTree.t L.t) (uf2: UFD.t) p (v2: L.t) : bool :=
   | _ => true
   end.
 
-(* It is used only if (m2 ! p is None && uf2 ! p = None) *)
+(* unused: It is used only if (m2 ! p is None && uf2 ! p = None) *)
 Definition val_eqb_opt1 (m2: PTree.t L.t) (uf2: UFD.t) p (v1: L.t) : bool :=
   match (UFD.m uf2) ! p, m2 ! p with
   (* p is a singleton in uf2 and it is not mapped to anything but it
@@ -262,25 +294,60 @@ Definition val_eqb_opt1 (m2: PTree.t L.t) (uf2: UFD.t) p (v1: L.t) : bool :=
   | _, _ => true
   end.
 
-(* How to argue that it does not reject too much? *)
+(* Unused code *)
+(*   ufd.eqb (uf dm1) (uf dm2) *)
+(* UFD.geb *)
+(*   && PTree.beq L.beq (m dm1) (m dm2). *)
+
+(* Lemma beq_correct: forall dm1 dm2, beq dm1 dm2 = true -> eq dm1 dm2. *)
+(* Proof. *)
+(*   intros.  *)
+(*   unfold beq in H. eapply andb_true_iff in H as (A & B). *)
+(*   constructor. *)
+(*   eapply UFD.eqb_correct. auto. *)
+(*   intros. unfold get. *)
+(*   assert (REQ: (UFD.repr (uf dm1) p) = (UFD.repr (uf dm2) p)). *)
+(* UFD.eq *)
+(*   {  eapply UFD.eqb_correct in A. red in A. *)
+(*      setoid_rewrite <- UFD.sameclass_repr. *)
+
+(* (** TODO: we may need a more efficient implementation for this *)
+(* equality checking as it may be the bottleneck of the performance. The *)
+(* following code is an attempt but it does not satisfy the strict *)
+(* equality definition which requires that the union-find are also *)
+(* equivalent *) *)
+
+
+(* Keep in mind that even if (uf dm1) = (uf dm2), it does not mean
+that the representative of some region [r] in (uf dm1) is equal to the
+representative of [r] in (uf dm2). *)
 Definition beq (dm1 dm2: t) : bool :=
   (* uf1 is included in uf2 *)
   UFD.geb (uf dm2) (uf dm1)
-  (* uf2 is included in uf1 and all the values of representative nodes
-  are equal *)
+  (* uf2 is included in uf1 and all the values of representative nodes *)
+  (* are equal *)
   && PTree_Properties.for_all (UFD.m (uf dm2)) (eqb_elt dm1 dm2)
-  (* If the node is a singleton in dm2 (which is not checked in the
-  previous for_all predicate), we need to check that they store the same
-  value in the map *)
+  (* If the node is a singleton in dm2 (which is not checked in the *)
+  (* previous for_all predicate), we need to check that they store the same *)
+  (* value in the map *)
   && PTree_Properties.for_all (m dm2) (val_eqb_opt2 (m dm1) (uf dm2))
   && PTree_Properties.for_all (m dm1) (val_eqb_opt1 (m dm2) (uf dm2)).
 
 Lemma beq_correct: forall dm1 dm2, beq dm1 dm2 = true -> eq dm1 dm2.
 Proof.
   intros dm1 dm2 EQ. unfold beq in EQ.
-  red. intros. unfold get.
   erewrite !andb_true_iff in EQ. destruct EQ as (((A & B) & C) & D).
-    destruct (PTree.get p (UFD.m (uf dm2))) eqn: G.
+  constructor.
+  assert (E: UFD.geb (uf dm1) (uf dm2) = true).
+  { unfold UFD.geb.
+    eapply PTree_Properties.for_all_correct.
+    intros.
+    eapply PTree_Properties.for_all_correct in B.
+    unfold eqb_elt in B. eapply andb_true_iff in B as (C1 & C2). eapply C1.
+    eauto. }
+  eapply UFD.eqb_correct. eapply andb_true_iff; eauto.
+  intros. unfold get.  
+  destruct (PTree.get p (UFD.m (uf dm2))) eqn: G.
   - eapply PTree_Properties.for_all_correct in G. 2: eauto.
     unfold eqb_elt, beq_elt in G. eapply andb_true_iff in G as (C1 & C2).
     destruct ((m dm1) ! (UFD.repr (uf dm1) p)) eqn: D1;
@@ -329,19 +396,27 @@ Proof.
             unfold val_eqb_opt1 in M1. rewrite G in M1.
             rewrite M2 in M1. congruence.
          ++ apply L.eq_refl.
-Qed.              
+Qed.
 
-Definition ge (x y: t) : Prop :=
-  forall p, L.ge (get p x) (get p y).
+Record ge' (x y: t) : Prop :=
+  { uf_ge: UFD.ge (uf x) (uf y);
+    m_ge: forall p, L.ge (get p x) (get p y) }.
+
+Definition ge := ge'.
 
 Lemma ge_refl: forall x y, eq x y -> ge x y.
 Proof.
-  unfold ge, eq; intros. apply L.ge_refl. auto.
+  intros. inv H.
+  constructor.
+  eapply UFD.ge_refl. auto.
+  intros. apply L.ge_refl. auto.
 Qed.
 
 Lemma ge_trans: forall x y z, ge x y -> ge y z -> ge x z.
 Proof.
-  unfold ge; intros. apply L.ge_trans with (get p y); auto.
+  intros. inv H; inv H0. constructor.
+  eapply UFD.ge_trans; eauto.
+  intros. apply L.ge_trans with (get p y); auto.
 Qed.
 
 Definition bot : t := mk (PTree.empty _) UFD.empty.
@@ -353,7 +428,9 @@ Qed.
 
 Lemma ge_bot: forall x, ge x bot.
 Proof.
-  unfold ge; intros. rewrite get_bot. apply L.ge_bot.
+  intros. constructor.
+  simpl. eapply UFD.ge_empty.
+  intros. rewrite get_bot. apply L.ge_bot.
 Qed.
 
 
@@ -443,7 +520,9 @@ Definition lub (dm1 dm2: t) : t :=
 
 Lemma ge_lub_left: forall x y, ge (lub x y) x.
 Proof.
-  intros dm1 dm2. red. intros.
+  intros dm1 dm2. constructor. 
+  unfold lub. simpl. eapply UFD.join_ge1.
+  intros.
   unfold get, lub. simpl.
   destruct ((m dm1) ! (UFD.repr (uf dm1) p)) eqn: G1.
   2: { eapply L.ge_bot. }
@@ -461,7 +540,9 @@ Qed.
   
 Lemma ge_lub_right: forall x y, ge (lub x y) y.
 Proof.
-  intros dm1 dm2. red. intros.
+  intros dm1 dm2. constructor. 
+  unfold lub. simpl. eapply UFD.join_ge2.
+  intros.
   unfold get, lub. simpl.
   destruct ((m dm2) ! (UFD.repr (uf dm2) p)) eqn: G2.
   2: { eapply L.ge_bot. }
@@ -710,6 +791,23 @@ Module LoansEnv <: SEMILATTICE.
   Axiom ge_lub_right: forall x y, ge (lub x y) y.
 
 End LoansEnv.
+
+Global Instance LOrgEnv_set_Proper: Proper (eq ==> LOrgSt.eq ==> LOrgEnv.eq ==> LOrgEnv.eq) LOrgEnv.set.
+Proof.
+  intros r1 r2 A ls1 ls2 B le1 le2 C. subst.
+  inv C. 
+  constructor.
+  unfold LOrgEnv.set.
+  destruct ls1; destruct ls2; simpl in *; eauto.
+  intros. rewrite !LOrgEnv.gsspec.
+  destruct peq.
+  - eapply uf_eq in e. rewrite e. rewrite peq_true. auto.
+  - destruct peq.
+    eapply uf_eq in e. unfold UFD.sameclass in e. rewrite e in n. congruence.
+    auto.
+Qed.  
+
+
 
 (* (* Update Alias graph *) *)
 
